Progress on PKAE interface

secure_api/box/functor_box/Box.PKAE.fst
@@ -30,23 +30,31 @@ module ID = Box.Indexing
 module ODH = Box.ODH
 module AE = Box.AE
 
-#set-options "--z3rlimit 1900 --max_ifuel 1 --max_fuel 0"
-abstract noeq type pkae_module =
-  | PKAE:
-    im:ID.index_module{ID.get_subId im == ODH.dh_share} ->
-    pm:Plain.plain_module{Plain.get_plain pm == AE.ae_plain} ->
-    am:AE.ae_module im pm ->
-    km:Key.key_module im{km == AE.instantiate_km am} ->
-    om:ODH.odh_module im km ->
-    pkae_module
+let nonce = AE.nonce
+let cipher = AE.cipher
 
-type skey = ODH.skey
-type pkey = ODH.pkey
-type nonce = AE.nonce
+let pkey = ODH.pkey
+let skey = ODH.skey
+
+#set-options "--z3rlimit 1900 --max_ifuel 1 --max_fuel 0"
+private noeq type box_pkae_module =
+  | BP:
+    pkm:pkae_module{ID.get_subId pkm.im == ODH.dh_share /\ Plain.get_plain pkm.pm == AE.ae_plain} ->
+    am:AE.ae_module pkm.im pkm.pm ->
+    km:Key.key_module pkm.im{km == AE.instantiate_km am} ->
+    om:ODH.odh_module pkm.im km ->
+    box_pkae_module
+
+let get_message_log pkm =
+  pkm.message_log
+
 type key (pkm:pkae_module) = AE.key pkm.im
-type id (pkm:pkae_module) = ID.id pkm.im
-type message (pkm:pkae_module) (i:id pkm) = AE.ae_protected_plain pkm.im pkm.pm i
-type cipher = AE.cipher
+
+let zero_bytes = AE.create_zero_bytes
+
+let nonce_is_fresh (pkm:pkae_module) (i:id pkm) (n:nonce) (h:mem) =
+  MR.m_contains pkm.message_log h
+  /\ MM.fresh pkm.message_log (n,i) h
 
 val gen: pkm:pkae_module -> ST (pkey*skey)
   (requires (fun h0 -> True))
@@ -54,7 +62,6 @@ val gen: pkm:pkae_module -> ST (pkey*skey)
 let gen pkm =
   ODH.keygen()
 
-let fresh pkm i = ID.fresh pkm.im (ID.ID i)
 let registered pkm i = ID.registered pkm.im (ID.ID i)
 let honest pkm i = ID.honest pkm.im (ID.ID i)
 let dishonest pkm i = ID.dishonest pkm.im (ID.ID i)
@@ -63,7 +70,7 @@ let dishonest pkm i = ID.dishonest pkm.im (ID.ID i)
 val encrypt: pkm:pkae_module -> #i:id pkm -> n:nonce -> sk:skey -> pk:pkey{ODH.compatible_keys sk pk /\ i = ID.compose_ids pkm.im (ODH.pk_get_share pk) (ODH.sk_get_share sk)} -> m:message pkm i{Plain.length #pkm.im #pkm.pm #i m / Spec.Salsa20.blocklen < pow2 32} -> ST cipher
   (requires (fun h0 ->
     registered pkm i
-    /\ AE.nonce_is_fresh pkm.am i n h0
+    /\ nonce_is_fresh pkm i n h0
     /\ Key.invariant pkm.im pkm.km h0
   ))
   (ensures  (fun h0 c h1 ->
@@ -77,6 +84,15 @@ let encrypt pkm #i n sk pk m =
   let c = AE.encrypt pkm.am #i n k m in
   c
 
-//
-//
-//val decrypt: pkm:pkae_module -> #i:id pkm -> n:nonce -> k:key pkm -> c:cipher -> option (message pkm i)
+val decrypt: pkm:pkae_module -> #i:id pkm -> n:nonce -> sk:skey -> pk:pkey{ODH.compatible_keys sk pk /\ i = ID.compose_ids pkm.im (ODH.pk_get_share pk) (ODH.sk_get_share sk)} -> c:cipher -> ST (option (message pkm i))
+  (requires (fun h0 ->
+    registered pkm i
+    /\ Key.invariant pkm.im pkm.km h0
+  ))
+  (ensures  (fun h0 c h1 ->
+    Key.invariant pkm.im pkm.km h1
+  ))
+let decrypt pkm #i n sk pk c =
+  let k = ODH.prf_odh pkm.im pkm.km pkm.om sk pk in
+  let m = AE.decrypt pkm.am #i n k c in
+  m
