secure_api/box/functor_box/Box.PKAE.fsti
@@ -1,0 +1,108 @@
+module Box.PKAE
+
+
+open FStar.Set
+open FStar.HyperHeap
+open FStar.HyperStack
+open FStar.HyperStack.ST
+open FStar.Monotonic.RRef
+open FStar.Seq
+open FStar.Monotonic.Seq
+open FStar.List.Tot
+
+open Crypto.Symmetric.Bytes
+
+open Box.Flags
+
+module MR = FStar.Monotonic.RRef
+module MM = MonotoneMap
+module HS = FStar.HyperStack
+module HH = FStar.HyperHeap
+module Plain = Box.Plain
+module ID = Box.Indexing
+
+
+type index_module = ID.index_module
+type plain_module = Plain.plain_module
+type id (im:index_module) = ID.id im
+val nonce: t:Type0{hasEq t}
+val cipher: Type0
+type log_region (im:index_module) =
+  r:MR.rid{disjoint r (ID.get_rgn im)}
+
+
+type message_log_key (im:index_module) = (nonce*(i:id im))
+type message_log_value (im:index_module) (pm:plain_module) (i:id im) = (cipher*Plain.protected_plain_t im (Plain.get_plain pm) i)
+let message_log_range (im:index_module) (pm:plain_module) = fun (k:message_log_key im) -> (message_log_value im pm (snd k))
+let message_log_inv (im:index_module) (pm:plain_module) (f:MM.map' (message_log_key im) (message_log_range im pm)) = True
+type message_log (im:index_module) (rgn:log_region im) (pm:plain_module) =
+  MM.t rgn (message_log_key im) (message_log_range im pm) (message_log_inv im pm)
+
+val pkey: Type0
+val skey: Type0
+
+noeq type pkae_module =
+  | PKAE:
+    im:ID.index_module ->
+    pm:Plain.plain_module ->
+    rgn:log_region im ->
+    enc: ((Plain.get_plain pm) -> n:nonce -> pk:pkey -> sk:skey -> Tot cipher) ->
+    dec: (c:cipher -> n:nonce -> pk:pkey -> sk:skey -> Tot (option (Plain.get_plain pm))) ->
+    message_log: message_log im rgn pm ->
+    pkae_module
+
+val get_message_log: pkm:pkae_module -> GTot (message_log pkm.im pkm.rgn pkm.pm)
+
+val zero_bytes: (n:nat) -> b:bytes{Seq.length b = n /\ b=Seq.create n (UInt8.uint_to_t 0)}
+
+val pkey_to_subId: #im:index_module -> pk:pkey -> ID.get_subId im
+val pkey_to_subId_inj: #im:index_module -> pk:pkey -> Lemma
+  (requires True)
+  (ensures (forall pk' . pkey_to_subId #im pk == pkey_to_subId #im pk' <==> pk == pk'))
+  [SMTPat (pkey_to_subId #im pk)]
+
+#set-options "--z3rlimit 2000 --max_ifuel 1 --max_fuel 0"
+val nonce_is_fresh: (pkm:pkae_module) -> (i:id pkm.im) -> (n:nonce) -> (h:mem) ->
+  (t:Type0{t <==>
+    (MR.m_contains pkm.message_log h
+    /\ MM.fresh pkm.message_log (n,i) h)})
+
+val pkey_from_skey: sk:skey -> pk:pkey
+
+val pkey_from_skey_inj: sk:skey -> pk:pkey -> Lemma
+  (requires True)
+  (ensures (forall sk1 sk2 . pkey_from_skey sk1 == pkey_from_skey sk2 <==> sk1 == sk2))
+
+val gen: unit -> ST (keypair:(pkey*skey){fst keypair == pkey_from_skey (snd keypair)})
+  (requires (fun h0 -> True))
+  (ensures (fun h0 _ h1 ->
+    modifies_none h0 h1
+  ))
+
+let registered pkm i = ID.registered pkm.im (ID.ID i)
+let honest pkm i = ID.honest pkm.im (ID.ID i)
+let dishonest pkm i = ID.dishonest pkm.im (ID.ID i)
+
+val compatible_keys: sk:skey -> pk:pkey -> t:Type0{t <==> pk =!= pkey_from_skey sk}
+
+val encrypt: pkm:pkae_module ->
+             #i:id pkm.im ->
+             n:nonce ->
+             sk:skey ->
+             pk:pkey{compatible_keys sk pk /\ i = ID.compose_ids pkm.im (pkey_to_subId #pkm.im pk) (pkey_to_subId #pkm.im (pkey_from_skey sk))} ->
+             m:(Plain.protected_plain_t pkm.im (Plain.get_plain pkm.pm) i) ->
+             ST cipher
+  (requires (fun h0 ->
+    registered pkm i
+    /\ nonce_is_fresh pkm i n h0
+  ))
+  (ensures  (fun h0 c h1 ->
+    ((honest pkm i /\ b2t ae_ind_cpa) // Ideal behaviour if the id is honest and the assumption holds.
+               ==> (c == pkm.enc (zero_bytes (Plain.length #pkm.im #pkm.pm #i m)) n pk sk))
+    /\ ((dishonest pkm i \/ ~(b2t ae_ind_cpa)) // Concrete behaviour otherwise.
+                  ==> (eq2 #cipher c (pkm.enc (Plain.repr #pkm.im #pkm.pm #i m) n pk sk)))
+    /\ ((honest pkm i) ==> // A message is added to the log if the id is honest. This also guarantees nonce-uniqueness.
+                      (MR.m_contains pkm.message_log h1
+                      /\ MR.witnessed (MM.contains pkm.message_log (n,i) (c,m))
+                      /\ MR.m_sel h1 pkm.message_log == MM.upd (MR.m_sel h0 pkm.message_log) (n,i) (c,m)))
+  ))
